TRUMP.dfy
@@ -1,4 +1,5 @@
-include "Ownership-Recursive.dfy"
+//include "Ownership-Recursive.dfy"
+include "Ownership-Parallel.dfy"
 
 
 
@@ -10,6 +11,48 @@ lemma fromTheManyOne(less : seq<nat>, more : seq<nat>)
 
 function sum(s : seq<int>) : int
   { if (|s| == 0) then 0 else s[0] + sum(s[1..]) }
+
+
+
+//
+//
+// lemma smooveOwnerator(divot : Owner, pivot : Owner, rivet : Owner, blivet : Owner, m : Klon)
+//  //given that pivot is cloned to blivet
+//  //lets see if partitioning owners across the pivot works
+//    requires AllReady(divot)
+//    requires AllReady(pivot)
+//    requires AllReady(rivet)
+//    requires AllReady(blivet)
+//
+//    requires klonReady(m)
+//    requires klonCalid(m)
+//
+//    requires flatten(divot) >= flatten(pivot)
+//    requires divot <= m.m.Keys
+//    requires pivot <= m.m.Keys
+//
+//    requires mapThruKlon(divot, m) == rivet
+//    requires mapThruKlon(pivot, m) == blivet
+//
+//     ensures flatten(rivet) >= flatten(blivet)
+//
+// {
+//       assert klonCalid(m);
+//       assert klonAllLines(m);
+//
+//
+//       assert flatten(rivet) >= flatten(blivet);
+// }
+//
+
+
+
+
+
+
+
+
+
 
 
 lemma smooveKlonerator(divot : Object, pivot : Object, rivet : Object, blivet : Object, m : Klon)
@@ -26,8 +69,6 @@ lemma smooveKlonerator(divot : Object, pivot : Object, rivet : Object, blivet : 
    requires pivot  == m.o
    requires blivet == m.c
 
-
-
    requires strictlyInside(divot, pivot)
    requires m.objectInKlown(divot)
    requires m.m[pivot] == blivet   //is this too much already?
@@ -43,18 +84,108 @@ lemma smooveKlonerator(divot : Object, pivot : Object, rivet : Object, blivet : 
       assert strictlyInside(divot, pivot);
       assert divot != pivot;
       assert klonIdentity(divot,rivet,m);
-
+      assert divot.AMFO <= m.m.Keys;
+      assert forall o <- divot.AMFO :: klonLine(o,m.m[o],m);
       assert mapThruKlon(divot.owner, m) == rivet.owner;
+
+ var divotInside,divotOutside,divotFringe := splitOwnersAroundPivot(divot, pivot);
+ assert pivot in divotFringe;
+ var divotFringeNoPivot := divotFringe - {pivot};
+
+ var rivetInside,rivetOutside,rivetFringe := splitOwnersAroundPivot(rivet, blivet);
+ assert blivet in rivetFringe;
+ var rivetFringeNoPivot := rivetFringe - {blivet};
+
+assert forall o <- divotInside :: && (o in m.m.Keys);
+assert forall o <- divotInside :: && (klonLine(o,m.m[o],m));
+
+// assert forall o <- divotInside :: && (m.m[o] in rivetInside);  //ERR GRRR
+
+assert divot.AMFO   >= pivot.AMFO;
+
+
+assert forall d <- divotFringeNoPivot :: not(strictlyInside(d,pivot));
+assert divotFringeNoPivot <= m.m.Keys;
+assert forall d <- divotFringeNoPivot :: klonLine(d,m.m[d],m);
+assert forall d <- divotFringeNoPivot :: m.m[d] == d;
+
+
+
+// assert forall d <- divotFringeNoPivot :: d in rivetFringeNoPivot;  //ERR GRRR
+// assert forall d <- rivetFringeNoPivot :: d in divotFringeNoPivot;  //ERR GRRR
+//
+// //  assert forall d <- divotInside :: m.m[d] in rivetInside;
+//  assert divotFringeNoPivot == rivetFringeNoPivot;                   //ERR GRRR
+
+
+
+}
+
+//
+// lemma KlonSplit(divot : Object, rivet : Object, m : Klon)
+// //part is sstrictly inside pivot AND so is whole (sob)
+//   requires part.Ready()
+//   requires pivot.Ready()
+//   requires whole.Ready()
+//   requires strictlyInside(part, pivot)
+//   requires strictlyInside(whole, pivot)
+//   requires inside(part, whole)
+// {
+//    var partInside,partOutside,partFringe    := splitOwnersAroundPivot(part, pivot);
+//    var wholeInside,wholeOutside,wholeFringe := splitOwnersAroundPivot(whole, pivot);
+//
+//    assert part.AMFO   >= whole.AMFO;
+//    assert partInside  >= wholeInside;
+//    assert partOutside >= wholeOutside;  //seems odd, but remember ?outside? is the upwarads closure of owners beyond the pivot.
+//    assert partFringe  >= wholeFringe;
+// }
+
+lemma SuperSplit(part : Object, pivot : Object, whole : Object)
+//part is sstrictly inside pivot AND so is whole (sob)
+  requires part.Ready()
+  requires pivot.Ready()
+  requires whole.Ready()
+  requires strictlyInside(part, pivot)
+  requires strictlyInside(whole, pivot)
+  requires inside(part, whole)
+{
+   var partInside,partOutside,partFringe    := splitOwnersAroundPivot(part, pivot);
+   var wholeInside,wholeOutside,wholeFringe := splitOwnersAroundPivot(whole, pivot);
+
+   assert part.AMFO   >= whole.AMFO;
+   assert partInside  >= wholeInside;
+   assert partOutside >= wholeOutside;  //seems odd, but remember ?outside? is the upwarads closure of owners beyond the pivot.
+   assert partFringe  >= wholeFringe;
 }
 
 
-
-
+//
+// lemma superJoin(part : Object, pivot : Object, whole : Object,
+//                 partInside : Owner, partOutside : Owner, partFringe : Owner,
+//                 wholeInside : Owner, wholeOutside : Owner, wholeFringe : Owner)
+// ///likely unuseable, but...
+//   requires part.Ready()
+//   requires pivot.Ready()
+//   requires whole.Ready()
+//   requires AllReady(partInside)
+//   requires AllReady(partOutside)
+//   requires AllReady(partFringe)
+//   requires AllReady(wholeInside)
+//   requires AllReady(wholeOutside)
+//   requires AllReady(wholeFringe)
+//
+//
+//   requires strictlyInside(part, pivot)  //grr
+//   requires strictlyInside(whole, pivot) //grr
+//
+//    ensures inside(part, whole) //note not strictly
+// {}
 
 lemma splitOwnersAroundPivot(part : Object, pivot : Object) returns (allInside : Owner, allOutside : Owner, fringe : Owner)
   //splits part.AMFO into the bits inside pivot,
   //the bits outside pivot,
   //and the fringe (bits outside that are direct owners of an owner inside...)
+  //FUCK,. shoudl this be a function?  or indeed series of functions?
   requires part.Ready()
   requires pivot.Ready()
   requires strictlyInside(part, pivot)
@@ -70,6 +201,12 @@ lemma splitOwnersAroundPivot(part : Object, pivot : Object) returns (allInside :
    ensures fringe == set x <- allInside, xo <- x.owner | (xo in allOutside)  :: xo
    ensures forall x <- fringe :: x in allOutside
    ensures flatten(fringe) == allOutside
+   ensures pivot in fringe
+   ensures (fringe - {pivot}) == set x <- allInside, xo <- x.owner | (xo in allOutside) && (xo != pivot) :: xo
+   ensures flatten(fringe - {pivot}) + flatten({pivot}) == flatten(fringe) == allOutside
+
+   //ensures part.AMFO == recOwners(part)  //can do with Axioms from Ownership-Parallel if necessary...
+
   {
    var all := part.AMFO;
 
@@ -130,7 +267,10 @@ lemma splitOwnersAroundPivot(part : Object, pivot : Object) returns (allInside :
   var flatFringeNoPivot := flatten(fringeNoPivot);
   assert pivot !in flatFringeNoPivot;
 
-  assert flatten(fringe - {pivot}) + flatten({pivot}) == flatten(fringe);
+  assert fringeNoPivot == set x <- allInside, xo <- x.owner | (xo in allOutside) && (xo != pivot) :: xo;
+
+  assert (fringe - {pivot}) == set x <- allInside, xo <- x.owner | (xo in allOutside) && (xo != pivot) :: xo;
+  assert flatten(fringe - {pivot}) + flatten({pivot}) == flatten(fringe) == allOutside;
 }
 
 
@@ -328,3 +468,164 @@ ghost function {:isolate_assertions} YouCan'tGetThereFromHereBut(part : Object, 
 //   assert not(inside(part, whole));
 //
 //   assert pivotlyOutside(part, whole) == not(strictlyInside(part, whole));
+
+lemma Flatten3(a : Owner, b : Owner, c : Owner)
+  // requires AllReady(a)
+  // requires AllReady(b)
+  // requires AllReady(c)
+  requires forall o <- a :: o.Ready()
+  requires forall o <- b :: o.Ready()
+  requires forall o <- c :: o.Ready()
+
+    requires a + b == c
+    ensures flatten(a) + flatten(b) == flatten(c)
+    ensures flatten(a) + flatten(b) == flatten(a+b)
+    ensures recFlatten(a)+recFlatten(b)==recFlatten(a+b)
+    {}
+
+lemma FLATTEN_SUMS(a : Owner, b : Owner, c : Owner, m : Klon)
+   requires a+b == c
+  // requires forall o <- a :: o.Ready()  //I'm OH SO TORY
+  // requires forall o <- b :: o.Ready()  //I'm OH SO TORY
+  // requires forall o <- c :: o.Ready()  //TORY TORY TORY
+  //  requires AllReady(a)
+  //  requires AllReady(b)
+  //  requires AllReady(c)
+  //  requires klonReady(m)
+  //  requires klonCalid(m)
+   requires (a+b+c) <= m.m.Keys
+//    ensures recFlatten(a)+recFlatten(b)==recFlatten(a+b)
+    ensures flatten(a) + flatten(b) == flatten(a+b)
+    ensures mapThruKlon(a,m) + mapThruKlon(b,m) == mapThruKlon(a+b,m)
+    ensures flatten(mapThruKlon(a,m)) + flatten(mapThruKlon(b,m)) == flatten(mapThruKlon(a+b,m))
+   {}
+
+lemma FLATTEN_ONE(o : Object)
+ requires o.Ready()
+ ensures flatten({o}) == {o} + flatten(o.owner) == o.AMFO
+ {}
+
+
+lemma {:timeLimit 20} MAPPEN_ONE(next : Object, m : Klon)
+  requires next.Ready()
+  requires next in m.m.Keys
+  requires klonReady(m)
+  requires klonCalid(m)
+   ensures mapThruKlon({next},m) == {m.m[next]}
+//   ensures flatten({next}) == {next} + flatten(next.owner)
+//   ensures flatten(mapThruKlon(done+{next},m)) == flatten(mapThruKlon(done,m)) + flatten(mapThruKlon({next},m))
+{
+    FLATTEN_ONE(next);
+//  assert mapThruKlon({next},m) == (set o <- {next} :: m.m[o]) == {m.m[next]};
+}
+
+lemma {:timeLimit 20} FLATTEN_TWO(done : Owner, next : Object, m : Klon)
+  requires AllReady(done)
+  requires next.Ready()
+  requires klonReady(m)
+  requires klonCalid(m)
+  requires (done+{next}) <= m.m.Keys
+   ensures (done+{next} == done + {next})
+   ensures mapThruKlon(done+{next},m) == mapThruKlon(done,m) + mapThruKlon({next},m)
+   ensures flatten(done+{next}) == flatten(done) + flatten({next})
+   ensures flatten(mapThruKlon(done+{next},m)) == flatten(mapThruKlon(done,m)) + flatten(mapThruKlon({next},m))
+{
+  FLATTEN_SUMS(done,{next},done+{next},m);
+}
+
+
+
+
+lemma recSplatten(oo : Owner, m : Klon) returns (sp : Owner)
+  decreases allAMFOs(oo)
+   requires AllReady(oo)
+   requires klonReady(m)
+   requires klonCalid(m)
+   requires oo <= m.m.Keys
+//
+//    requires |oo| == 1
+//    requires forall o <- oo :: o.owner == {}
+//     ensures flatten(oo) == oo
+
+    ensures flatten(oo) <= m.m.Keys
+    ensures sp == flatten(mapThruKlon(oo, m))
+   {
+//     var x :=  {set o : Object <- oo, ooo <- recOwners(o) :: ooo};
+
+    sp := {};
+
+    var todo := oo;
+    var done : Owner := {};
+    assert AllReady(todo);
+    assert oo - todo == {};
+    assert mapThruKlon({}, m) == {};
+    assert mapThruKlon((oo - todo), m) == {};
+    assert flatten({}) == {};
+    assert flatten(mapThruKlon((oo - todo), m)) == {};
+
+    assert sp == flatten(mapThruKlon((oo - todo), m));
+    assert done == oo - todo == {};
+    assert sp == flatten(mapThruKlon((done), m));
+
+    while (todo > {})
+        decreases todo
+        invariant sp == flatten(mapThruKlon((oo - todo), m))
+        invariant done == oo - todo
+        invariant sp == flatten(mapThruKlon((done), m))
+          {
+            assert sp == flatten(mapThruKlon((oo - todo), m));
+            var next :| next in todo;
+            assert done == oo - todo;
+            assert done + {next} == oo - (todo - {next});
+            todo := todo - {next};
+            assert done + {next} == oo - todo;
+
+            var sext := m.m[next];
+            assert klonLine(next, sext, m);
+            assert klonIdentity(next, sext, m);
+
+            var sowner;   var fowner;
+
+            if (next == m.o)
+              {
+                assert sext == m.c;
+                sowner := m.clowner;
+                fowner := flatten(m.clowner);
+                assert fowner == flatten(sext.owner);
+              }
+            else if (outside(next, m.o))
+              {
+                assert next == sext; assert next.owner == sext.owner;
+                sowner := next.owner;
+                fowner := flatten(next.owner);
+                assert fowner == flatten(sext.owner);
+              }
+            else
+              {
+                assert strictlyInside(next, m.o);
+                sowner := mapThruKlon(next.owner, m);
+                assert sowner == sext.owner;
+                fowner := recSplatten(next.owner, m);
+                assert fowner == flatten(sext.owner);
+              } //end if elseif else
+
+            assert fowner == flatten(sext.owner);
+            FLATTEN_ONE(sext);
+            assert flatten({sext}) == ({sext} + flatten(sext.owner)) == ({sext} + fowner);
+            MAPPEN_ONE(next,m);
+            assert mapThruKlon({next}, m) == {m.m[next]} == {sext};
+            assert flatten(mapThruKlon({next}, m)) == flatten({sext}) == ({sext} + fowner);
+            assert sp == flatten(mapThruKlon((done), m));
+            assert (done+{next}) == (done)+({next});    FLATTEN_SUMS(done,{next},done+{next},m);
+            assert (mapThruKlon((done+{next}), m)) == (mapThruKlon((done), m)) + (mapThruKlon(({next}), m));
+            assert flatten(mapThruKlon((done+{next}), m)) == flatten(mapThruKlon((done), m)) + flatten(mapThruKlon(({next}), m)) == sp + ({sext} + fowner);
+            sp := sp + ({sext} + fowner);
+            done := done + {next};
+            assert done == oo - todo;
+            assert sp == flatten(mapThruKlon((done), m));
+            assert sp == flatten(mapThruKlon((oo - todo), m));
+          }//end while
+      assert sp == flatten(mapThruKlon((oo - todo), m));
+      assert todo == {}; assert done == oo;
+      assert sp == flatten(mapThruKlon(oo, m));
+  }
